src/testcases/cager/jexpr/linkuni.bpl
@@ -1,0 +1,108 @@
+type Ref;
+const null: Ref;
+
+var val: [Ref]int;
+var next: [Ref]Ref;
+var packedRange: [Ref] bool;
+var fracRange: [Ref] real;
+var packedUniRange: [Ref] bool;
+var fracUniRange: [Ref] real;
+
+procedure ConstructLink(val1 :int, next1 : Ref, this: Ref);
+	 ensures (val[this] == val1) &&
+ 	 	 (next[this] == next1); 
+ 
+procedure PackRange(x:int, y:int, this:Ref);
+	 requires packedRange[this]==false &&
+	 	((((val[this]>=x))&&(val[this]<=y))&&((fracRange[next[this]] > 0.0)||(next[this]==null)));
+
+procedure UnpackRange(x:int, y:int, this:Ref);
+	 requires packedRange[this] &&
+	 	 (fracRange[this] > 0.0);
+	 ensures ((((val[this]>=x))&&(val[this]<=y))&&((fracRange[next[this]] > 0.0)||(next[this]==null)));
+
+procedure PackUniRange(x:int, y:int, this:Ref);
+	 requires packedUniRange[this]==false &&
+	 	((((val[this]>=x))&&(val[this]<=y))&&(fracUniRange[next[this]] == 1.0||(next[this]==null)));
+
+procedure UnpackUniRange(x:int, y:int, this:Ref);
+	 requires packedUniRange[this] &&
+	 	 (fracUniRange[this] > 0.0);
+	 ensures ((((val[this]>=x))&&(val[this]<=y))&&(fracUniRange[next[this]] == 1.0||(next[this]==null)));
+
+procedure addModulo11(x:int,this:Ref)
+	 modifies fracRange,next,packedRange,val;
+	 requires ((x>=0)&&packedRange[this] && 
+ 	 	(fracRange[this] > 0.0));
+	 ensures packedRange[this] && 
+ 	 	(fracRange[this] > 0.0);
+requires (forall x0:Ref :: packedRange[x0]);
+	 ensures (forall x0:Ref:: (packedRange[x0] == old(packedRange[x0])));
+	 ensures (forall x0:Ref:: (fracRange[x0] == old(fracRange[x0])));
+
+{
+call UnpackRange(0, 10, this);
+packedRange[0, 10, this] := false;
+val[this]:=modulo(val[this]+x,11);
+call PackRange(0, 10, this);
+packedRange[0, 10, this] := true;
+if (next[this]!=null)
+{
+	 call addModulo11(x,next[this]);
+	fracRange[next[this]] := fracRange[next[this]] / 2.0;
+	fracRange[next[this]] := fracRange[next[this]] * 2.0;
+}
+ }
+ function modulo(x:int, y:int) returns (int); 
+axiom (forall x:int, y:int :: {modulo(x,y)}
+	 ((0 <= x) &&(0 < y) ==> (0 <= modulo(x,y) ) && (modulo(x,y) < y) )
+	&&
+	((0 <= x) &&(y < 0) ==> (0 <= modulo(x,y) ) && (modulo(x,y) < -y) )
+	&&
+	((x <= 0) &&(0 < y) ==> (-y <= modulo(x,y) ) && (modulo(x,y) <= 0) )
+	&&
+	((x <= 0) &&(y < 0) ==> (y <= modulo(x,y) ) && (modulo(x,y) <= 0) )
+	);
+
+procedure add(z:int,x:int,y:int,this:Ref)
+	 modifies fracUniRange,next,packedUniRange,val;
+	 requires ((x<y)&&packedUniRange[this] && 
+ 	 	(fracUniRange[this] == 1.0));
+	 ensures packedUniRange[this] && 
+ 	 	(fracUniRange[this] == 1.0);
+{
+call UnpackUniRange(x, y, this);
+packedUniRange[x, y, this] := false;
+val[this]:=val[this]+z;
+if (next[this]!=null)
+{
+	 call add(z,x,y,next[this]);
+	fracUniRange[next[this]] := fracUniRange[next[this]] / 2.0;
+	fracUniRange[next[this]] := fracUniRange[next[this]] * 2.0;
+}
+ call PackUniRange(x+z, y+z, this);
+packedUniRange[x+z, y+z, this] := true;
+}
+ procedure main(this:Ref)
+	 modifies fracRange,next,packedRange,val;
+requires (forall x:Ref :: packedRange[x]);
+{
+	 var l1:Ref;
+	 var l2:Ref;
+	 var l3:Ref;
+	 call ConstructLink(3,null,l1);
+packedRange[0,10,l1] := true;
+fracRange[0,10,l1] := 1.0;
+	 call ConstructLink(4,l1,l2);
+packedRange[0,10,l2] := true;
+fracRange[0,10,l2] := 1.0;
+	fracRange[l1] := fracRange[l1] / 2.0;
+	 call ConstructLink(5,l2,l3);
+packedRange[0,10,l3] := true;
+fracRange[0,10,l3] := 1.0;
+	fracRange[l2] := fracRange[l2] / 2.0;
+	 call addModulo11(20,l3);
+	fracRange[l3] := fracRange[l3] / 2.0;
+	fracRange[l3] := fracRange[l3] * 2.0;
+}
+ 
