src/testcases/cager/jexpr/share.bpl
@@ -1,0 +1,68 @@
+//----------------------------------
+//new class
+
+var dc: [Ref]Ref;
+var packedShareCount: [Ref] bool;
+var fracShareCount: [Ref] real;
+
+procedure ConstructShare(dc1 : Ref, this: Ref);
+	 ensures (dc[this] == dc1); 
+ 
+procedure PackShareCount(d:DoubleCount, this:Ref);
+	 requires packedShareCount[this]==false &&
+	 	(fracOK[dc[this]] == 0.1); 
+ 
+procedure UnpackShareCount(d:DoubleCount, this:Ref);
+	 requires packedShareCount[this] &&
+	 	 (fracShareCount[this] > 0.0);
+	 ensures (fracOK[dc[this]] == 0.1);
+
+procedure touch(this:Ref)
+	 modifies dbl,dc,fracOK,packedOK,packedShareCount,val;
+	 requires packedShareCount[this] && 
+ 	 	(fracShareCount[this] > 0.0);
+	 ensures packedShareCount[this] && 
+ 	 	(fracShareCount[this] > 0.0);
+	 requires (forall x:Ref :: packedShareCount[x]);
+	 requires (forall x:Ref :: packedOK[x]);
+	 ensures (forall x:Ref:: (packedOK[x] == old(packedOK[x])));
+	 ensures (forall x:Ref:: (fracOK[x] == old(fracOK[x])));
+
+	 ensures (forall x:Ref:: (packedShareCount[x] == old(packedShareCount[x])));
+
+{
+call UnpackShareCount(dc[this], this);
+packedShareCount[this] := false;
+	 call increment(this);
+	fracOK[this] := fracOK[this] / 2.0;
+	fracOK[this] := fracOK[this] * 2.0;
+call PackShareCount(dc[this], this);
+packedShareCount[this] := true;
+}
+ procedure main(this:Ref)
+	 modifies dbl,dc,fracOK,fracShareCount,packedOK,packedShareCount,val;
+	 requires (forall x:Ref :: packedShareCount[x]);
+	 requires (forall x:Ref :: packedOK[x]);
+{
+	 var dc0:Ref;
+	 var s1:Ref;
+	 var s2:Ref;
+	 call ConstructDoubleCount(2,4,dc0);
+packedOK[dc0] := true;
+fracOK[dc0] := 1.0;
+	 call ConstructShare(dc0,s1);
+packedShareCount[s1] := true;
+fracShareCount[s1] := 1.0;
+	fracOK[dc0] := fracOK[dc0] / 2.0;
+	 call ConstructShare(dc0,s2);
+packedShareCount[s2] := true;
+fracShareCount[s2] := 1.0;
+	fracOK[dc0] := fracOK[dc0] / 2.0;
+	 call touch(s1);
+	fracShareCount[s1] := fracShareCount[s1] / 2.0;
+	fracShareCount[s1] := fracShareCount[s1] * 2.0;
+	 call touch(s2);
+	fracShareCount[s2] := fracShareCount[s2] / 2.0;
+	fracShareCount[s2] := fracShareCount[s2] * 2.0;
+}
+ 
