src/testcases/cager/jexpr/simplecell.bpl
@@ -1,0 +1,82 @@
+type Ref;
+const null: Ref;
+
+var val: [Ref]int;
+var next: [Ref]Ref;
+var packedPredNext: [Ref] bool;
+var fracPredNext: [Ref] real;
+var packedPredVal: [Ref] bool;
+var fracPredVal: [Ref] real;
+
+procedure ConstructSimpleCell(val1 :int, next1 : Ref, this: Ref);
+	 ensures (val[this] == val1) &&
+ 	 	 (next[this] == next1); 
+ 
+procedure PackPredNext(obj: Ref, this:Ref);
+	 requires (packedPredNext[this]==false) &&
+	 	(((fracPredVal[next[this]] >= 0.34))) && (next[this]==obj); 
+ 
+procedure UnpackPredNext(obj: Ref, this:Ref);
+	 requires packedPredNext[this] &&
+	 	 (fracPredNext[this] > 0.0);
+	 ensures (((fracPredVal[next[this]] >= 0.34))) && (next[this]==obj);
+
+procedure PackPredVal(v:int, this:Ref);
+	 requires (packedPredVal[this]==false) &&
+	 	((v<15)) && (val[this]==v); 
+ 
+procedure UnpackPredVal(v:int, this:Ref);
+	 requires packedPredVal[this] &&
+	 	 (fracPredVal[this] > 0.0);
+	 ensures ((v<15)) && (val[this]==v);
+
+
+procedure changeVal(r:int, this:Ref)
+	 modifies packedPredVal,val;
+	 requires (this != null) && (((packedPredVal[this]) && 
+ 	 	(fracPredVal[this] >= 1.0))&&(r<15));
+	 ensures ((packedPredVal[this]) && 
+ 	 	(fracPredVal[this] >= 1.0));
+	 ensures (forall x:Ref :: packedPredVal[x]);
+	 ensures (forall x:Ref :: (fracPredVal[x]==old(fracPredVal[x])));
+
+{
+	 assume (forall y:Ref :: (fracPredVal[y] >= 0.0) );
+call UnpackPredVal(val[this], this);
+packedPredVal[this] := false;
+val[this]:=r;
+call PackPredVal(r, this);
+packedPredVal[this] := true;
+}
+ 
+procedure main(this:Ref)
+	 modifies fracPredNext,fracPredVal,packedPredNext,packedPredVal,val;
+	 requires (forall x:Ref :: packedPredNext[x]);
+	 requires (forall x:Ref :: packedPredVal[x]);
+{
+	 var c:Ref;
+	 var a:Ref;
+	 var b:Ref;
+	 assume (forall y:Ref :: (fracPredNext[y] >= 0.0) );
+	 assume (forall y:Ref :: (fracPredVal[y] >= 0.0) );
+	 call ConstructSimpleCell(c);
+packedPredVal[c] := true;
+fracPredVal[c] := 1.0;
+null, 	 call ConstructSimpleCell(a);
+packedPredNext[a] := true;
+fracPredNext[a] := 1.0;
+	fracPredVal[c] := fracPredVal[c] / 2.0;
+	 call ConstructSimpleCell(b);
+packedPredNext[b] := true;
+fracPredNext[b] := 1.0;
+	fracPredVal[c] := fracPredVal[c] / 2.0;
+call UnpackPredNext(c, a);
+fracPredVal[c] := fracPredVal[c] + 0.34;
+packedPredNext[a] := false;
+call UnpackPredNext(c, b);
+fracPredVal[c] := fracPredVal[c] + 0.34;
+packedPredNext[b] := false;
+fracPredVal[c] := fracPredVal[c]+0.34+0.34;
+	 call changeVal(4,c);
+}
+ 
